Coq/intrusive/lists/deque.v
@@ -7,7 +7,7 @@ Section Deque.
 (* ------------------ Representation predicate  ------------------- *)
 
   Definition pred l (vs: list val) : iProp Σ :=
-    ∃ L, DCycle.pred l L ∗ [∗ list] i ↦ l ; v ∈ L ; vs, (l +ₗ 2) ↦ v.
+    ∃ L, DCycle.pred l L ∗ [∗ list] i ↦ l ; v ∈ L ; vs, (l +ₗ (-1)) ↦ v.
   Notation is_deque := pred.
 
 (* --------------------- Functions on deques ---------------------- *)
@@ -18,26 +18,28 @@ Definition new : val :=
 
 Definition push_front : val :=
   λ: "x" "l", let: "l_x" := AllocN #3 "x" in
-    DCycle.insert_0 "l" "l_x".
+    DCycle.insert_0 "l" ("l_x" +ₗ #1).
 
 Definition push_back : val :=
   λ: "x" "l", let: "l_x" := AllocN #3 "x" in
-    DCycle.insert_1 "l" "l_x".
+    DCycle.insert_1 "l" ("l_x" +ₗ #1).
 
 Definition pop_front : val :=
-  λ: "l", if: DCycle.is_empty "l" then NONEV else
+  λ: "l",
+    if: DCycle.is_empty "l" then NONEV else
     let: "next" := DCycle.next "l" in
-    let: "x" := !("next" +ₗ #2) in
+    let: "x" := !("next" +ₗ #-1) in
     let: "rem" := DCycle.remove_0 "l" in
-    array_free "rem" #3 ;;
+    array_free ("rem" +ₗ #-1) #3 ;;
     SOME "x".
 
 Definition pop_back : val :=
-  λ: "l", if: DCycle.is_empty "l" then NONEV else
+  λ: "l",
+    if: DCycle.is_empty "l" then NONEV else
     let: "prev" := DCycle.prev "l" in
-    let: "x" := !("prev" +ₗ #2) in
+    let: "x" := !("prev" +ₗ #-1) in
     let: "rem" := DCycle.remove_1 "l" in
-    array_free "rem" #3;;
+    array_free ("rem" +ₗ #-1) #3;;
     SOME "x".
 
 (* ------------------- Verificiation of the Specs ----------------- *)
@@ -53,10 +55,10 @@ Lemma push_front_spec D (x: val) (l: loc) :
   push_front x #l
 {{{ RET #(); is_deque l (x :: D) }}}.
 Proof.
-  iStep 18 as (Φ L l') "HL HLD ? Hl'"; iModIntro.
-  rewrite unfold_array.
+  iStep 21 as (Φ L l') "HL HLD ? Hl'".
+  rewrite unfold_array; simpl.
   iDestruct "Hl'" as "[H0 [H1 H2]]".
-  wp_apply (DCycle.insert_0_spec with "[HL H0 H1]"); iSteps.
+  wp_apply (DCycle.insert_0_spec with "[HL H1 H2]"); iSteps.
 Qed.
 
 Lemma push_back_spec D (x: val) (l: loc) :
@@ -64,10 +66,10 @@ Lemma push_back_spec D (x: val) (l: loc) :
   push_back x #l
 {{{ RET #(); is_deque l (D ++ [x]) }}}.
 Proof.
-  iStep 18 as (Φ L' l') "HL HLD HΦ Hl"; iModIntro.
-  rewrite unfold_array.
+  iStep 21 as (Φ L' l') "HL HLD HΦ Hl".
+  rewrite unfold_array; simpl.
   iDestruct "Hl" as "[H0 [H1 H2]]".
-  wp_apply (DCycle.insert_1_spec with "[HL H0 H1]"); iSteps.
+  wp_apply (DCycle.insert_1_spec with "[HL H1 H2]"); iSteps.
   rewrite big_sepL2_app_same_length; auto; iSteps.
 Qed.
 
@@ -82,9 +84,9 @@ Lemma pop_front_cons_spec D (l: loc) (x: val) :
   pop_front #l
 {{{ RET (SOMEV x); is_deque l D }}}.
 Proof.
-  iSteps as (Φ l' L x0 x1) "HΦ HLD Hl'2 HL Hl'"; iModIntro.
+  iSteps as (Φ l' L x0 x1) "HΦ HLD Hl'2 HL Hl'".
   wp_apply (wp_array_free with "[Hl' Hl'2] [-]").
-  2: { instantiate (1:= [x0; x1; x]); iSteps. }
+  2: { instantiate (1:= [x; x0; x1]); iSteps. }
   all: reflexivity || iSteps.
 Qed.
 
@@ -106,10 +108,9 @@ Proof.
   iDestruct (big_sepL2_cons_inv_r with "HL2") as (l2 L3 ->) "[Hl2 HL2]".
   iDestruct (big_sepL2_nil_inv_r with "HL2") as "%H"; subst; iClear "HL2".
   iStep 10 as "Hl".
-  (* wp_apply (DCycle.prev_spec with "HL"); iIntros "HL". *)
-  rewrite rev_unit; simpl. iSteps as (x0 x1) "Pl2_2 Hl Pl2"; iModIntro.
+  rewrite rev_unit; simpl. iSteps as (x0 x1) "Pl2_2 Hl Pl2".
   wp_apply (wp_array_free with "[Pl2 Pl2_2] [-]").
-  2: { instantiate (1:= [x0; x1; x]); iSteps. }
+  2: { instantiate (1:= [x; x0; x1]); iSteps. }
   all: reflexivity || iSteps.
 Qed.
 
